Elevm/Types.lean
@@ -3,35 +3,65 @@
 import Elevm.Basic
 import Std.Data.TreeMap.Lemmas
 
-structure Adr : Type where
-  (high : B32)
-  (mid : B64)
-  (low : B64)
+
+def Adr : Type := B32 × B128
+
+
+
+structure Adr' : Type where
+  (high : UInt32)
+  (mid : UInt64)
+  (low : UInt64)
 deriving DecidableEq
 
-def Adr.toNat (x : Adr) : Nat :=
+def Adr'.toNat (x : Adr') : Nat :=
   x.high.toNat * (2 ^ 128) +
   x.mid.toNat * (2 ^ 64) +
   x.low.toNat
 
-def Nat.toAdr (n : Nat) : Adr :=
+def Adr.toNat (x : Adr) : Nat :=
+  (x.1.toNat <<< 128) ||| x.2.toNat
+
+def Nat.toAdr' (n : Nat) : Adr' :=
   {
     high := (n / (2 ^ 128)).toUInt32
     mid  := (n / (2 ^ 64)).toUInt64
     low  := n.toUInt64
   }
 
+def Nat.toAdr (n : Nat) : Adr :=
+  ⟨(n >>> 128).toB32, n.toB128⟩
+
 instance {n} : OfNat Adr n := ⟨n.toAdr⟩
 
-lemma Nat.toNat_toUInt32 {n : ℕ} : n.toUInt32.toNat = n % 2 ^ 32 :=
+lemma toNat_toB32 {n : ℕ} : B32.toNat n.toB32 = n ↾ 32 :=
   UInt32.toNat_ofNat
-lemma Nat.toNat_toUInt64 {n : ℕ} : n.toUInt64.toNat = n % 2 ^ 64 :=
+
+lemma toNat_toB64 {n : ℕ} : B64.toNat (n.toB64) = n ↾ 64 :=
   UInt64.toNat_ofNat
 
-lemma Nat.mod_two_pow_succ {k m} :
-    (k % (2 ^ (m + 1))) = (k / 2) % (2 ^ m) * 2 + k % 2 := by
-  rw [Nat.pow_succ, Nat.mul_comm, Nat.mod_mul]
-  rw [Nat.add_comm, Nat.mul_comm]
+lemma Nat.lo_lo_of_le {k m n : Nat} (le : m ≤ n) :
+    (k ↾ m) ↾ n = k ↾ m := mod_mod_of_dvd' <| Nat.pow_dvd_pow _ le
+
+lemma Nat.lo_lo_of_ge {k m n : Nat} (ge : m ≥ n) :
+    (k ↾ m) ↾ n = k ↾ n := mod_mod_of_dvd _ <| Nat.pow_dvd_pow _ ge
+
+lemma Nat.hi_or_lo (a b : Nat) : a ↿ b ||| a ↾ b = a := by
+  simp only [Nat.hi, Nat.lo]
+  rw [Nat.shiftLeft_eq, Nat.shiftRight_eq_div_pow]
+  rw [← @Nat.add_eq_or b, Nat.div_add_mod']
+  · apply Nat.dvd_mul_left
+  · apply Nat.mod_lt _ (Nat.pow_pos _); omega
+
+lemma Nat.or_eq_lo_add {k m n : Nat} :
+    (k >>> n ↾ m) <<< n ||| k ↾ n = k ↾ (m + n) := by
+  rw [← @Nat.lo_add_shr k m n]
+  rw [← @Nat.lo_lo_of_ge k (m + n) n (by omega)]
+  apply Nat.hi_or_lo
+
+lemma toNat_toB128 (n : Nat) : n.toB128.toNat = n ↾ 128 := by
+  simp only [Nat.toB128, B128.toNat]; rw [toNat_toB64, toNat_toB64]
+  apply Nat.or_eq_lo_add
 
 lemma Nat.div_two_pow_mod_two_pow (k m n : Nat) :
     (k / (2 ^ m)) % (2 ^ n) = (k % (2 ^ (m + n))) / (2 ^ m) := by
@@ -50,77 +80,856 @@ lemma Nat.div_two_pow_mod_two_pow (k m n : Nat) :
     · rw [Nat.mod_div_self, Nat.mul_div_cancel _ (by omega)]; rfl
     · simp [Nat.mul_mod_left, Nat.mod_lt]
 
-lemma Nat.toNat_toAdr (n : Nat) : n.toAdr.toNat = n % (2 ^ 160) := by
-  simp only [Nat.toAdr, Adr.toNat]
-  simp only [Nat.toNat_toUInt32, Nat.toNat_toUInt64]
-  simp only [Nat.div_two_pow_mod_two_pow]
-  rw [← @Nat.mod_mod_of_dvd (2 ^ 64) (2 ^ 128) n (Nat.pow_dvd_pow _ (by omega))]
-  rw [Nat.add_assoc, Nat.div_add_mod']
-  rw [← @Nat.mod_mod_of_dvd (2 ^ 128) (2 ^ 160) n (Nat.pow_dvd_pow _ (by omega))]
-  rw [Nat.div_add_mod']
+lemma Nat.toNat_toAdr (n : Nat) : n.toAdr.toNat = n ↾ 160 := by
+  simp only [Nat.toAdr, Adr.toNat]; rw [toNat_toB32, toNat_toB128]
+  apply Nat.or_eq_lo_add
+--
+-- lemma B64.toNat_mul_add_toNat_lt_size (x y : B64) :
+--     x.toNat * (2 ^ 64) + y.toNat < 2 ^ 128 := by
+--   have h : 2 ^ 128 = (UInt64.size - 1) * (2 ^ 64) + UInt64.size := by rfl
+--   rw [h]; clear h
+--   apply Nat.add_lt_add_of_le_of_lt _ (UInt64.toNat_lt_size _)
+--   apply Nat.mul_le_mul_right
+--   apply @Nat.le_pred_of_lt _ (UInt64.size) <| UInt64.toNat_lt_size _
 
 
-lemma Nat.add_div_of_dvd_of_dvd {a b c : ℕ} (ha : c ∣ a) (hb : c ∣ b) (hc : 0 < c) :
+lemma toB32_toNat {x : B32} : x.toNat.toB32 = x := UInt32.ofNat_toNat
+
+lemma toB32_or (a b : Nat) : (a ||| b).toB32 = a.toB32 ||| b.toB32 :=
+  UInt32.ofNat_or a b
+
+lemma toB64_or (a b : Nat) : (a ||| b).toB64 = a.toB64 ||| b.toB64 :=
+  UInt64.ofNat_or a b
+
+lemma B128.or_eq (x y : B128) :
+  x ||| y = ⟨x.1 ||| y.1, x.2 ||| y.2⟩ := rfl
+
+lemma toB128_or (a b : Nat) : (a ||| b).toB128 = a.toB128 ||| b.toB128 := by
+  simp only [Nat.toB128]
+  rw [B128.or_eq, toB64_or, Nat.shiftRight_or_distrib, toB64_or]
+
+lemma Nat.shiftLeft_lt_of_lt {a b n : Nat} (h : a < 2 ^ n) :
+    (a <<< b) < (2 ^ (n + b)) := by
+  rw [Nat.shiftLeft_eq, Nat.pow_add]
+  apply Nat.mul_lt_mul_of_pos_right h (Nat.pow_pos (by omega))
+
+lemma B128.toNat_lt {x : B128} : x.toNat < 2 ^ 128 := by
+  simp only [B128.toNat]; apply Nat.or_lt_two_pow
+  · apply Nat.shiftLeft_lt_of_lt B64.toNat_lt
+  · apply lt_trans B64.toNat_lt; omega
+
+lemma B256.toNat_lt (x : B256) : x.toNat < 2 ^ 256 := by
+  simp only [B256.toNat]; apply Nat.or_lt_two_pow
+  · apply Nat.shiftLeft_lt_of_lt B128.toNat_lt
+  · apply lt_trans B128.toNat_lt; omega
+
+lemma B64.zero_or {x : B64} : (0 ||| x) = x := UInt64.zero_or
+
+lemma B128.zero_or {x : B128} : (0 ||| x) = x := by
+  rw [B128.or_eq]; apply Prod.ext <;> {simp}
+
+lemma Nat.add_div_of_dvd {a b c : Nat} (c_pos : 0 < c) (c_dvd : c ∣ a)  :
     (a + b) / c = a / c + b / c := by
-  rw [Nat.add_div hc, if_neg]
-  · rfl
-  · rw [Nat.mod_eq_zero_of_dvd ha, Nat.mod_eq_zero_of_dvd hb]
-    intro h; cases lt_of_lt_of_le hc h
+  rw [Nat.add_div c_pos, if_neg, Nat.add_zero]
+  rw [not_le, Nat.mod_eq_zero_of_dvd c_dvd, Nat.zero_add]
+  apply Nat.mod_lt _ c_pos
 
-lemma Nat.add_div_of_dvd_of_lt {a b c : ℕ} (ha : c ∣ a) (hb : b < c) :
-    (a + b) / c = a / c + b / c := by
-  rw [Nat.add_div (zero_lt_of_lt hb), if_neg]
-  · rfl
-  · rw [Nat.mod_eq_zero_of_dvd ha, Nat.mod_eq_of_lt hb]; simp [hb]
+lemma Nat.div_eq_zero_of_lt {k x : Nat} (h : x < k) : x / k = 0 := by
+  rw [Nat.div_eq_zero_iff_lt (by omega)]; apply h
 
-lemma B64.toNat_mul_add_toNat_lt_size (x y : B64) :
-    x.toNat * (2 ^ 64) + y.toNat < 2 ^ 128 := by
-  have h : 2 ^ 128 = (UInt64.size - 1) * (2 ^ 64) + UInt64.size := by rfl
-  rw [h]; clear h
-  apply Nat.add_lt_add_of_le_of_lt _ (UInt64.toNat_lt_size _)
-  apply Nat.mul_le_mul_right
-  apply @Nat.le_pred_of_lt _ (UInt64.size) <| UInt64.toNat_lt_size _
+lemma Nat.add_div_of_dvd_of_lt' {a b c : Nat} (c_dvd : c ∣ a) (b_lt : b < c) :
+    (a + b) / c = a / c := by
+  rw [Nat.add_div_of_dvd (zero_lt_of_lt b_lt) c_dvd]
+  simp [Nat.div_eq_zero_of_lt b_lt]
 
-lemma Adr.toAdr_toNat (a : Adr) : a.toNat.toAdr = a := by
-  have aux : ∀ x : Nat, x * (2 ^ 128) = x * (2 ^ 64) * (2 ^ 64) := by
-    intro x; rw [Nat.mul_assoc]
+lemma toB64_add (a b : Nat) :
+    (a + b).toB64 = a.toB64 + b.toB64 := UInt64.ofNat_add a b
+
+lemma B64.lt_iff_toNat_lt {a b : B64} : a < b ↔ a.toNat < b.toNat :=
+  UInt64.lt_iff_toNat_lt
+
+lemma B64.toNat_add (a b : B64) : (a + b).toNat = (a.toNat + b.toNat) ↾ 64 :=
+  UInt64.toNat_add a b
+
+lemma Nat.lo_eq_of_lt {a b : ℕ} (h : a < (2 ^ b)) : a ↾ b = a :=
+  Nat.mod_eq_of_lt h
+
+lemma Nat.add_mod_eq_add_sub {k m n : Nat} (m_lt : m < k)
+    (n_lt : n < k) (k_le : k ≤ m + n) : (m + n) % k = m + n - k := by
+  rcases Nat.exists_eq_add_of_le k_le with ⟨d, eq⟩
+  rw [eq, Nat.add_mod_left]
+  have d_lt : d < k := by
+    rw [← @Nat.add_lt_add_iff_left k, ← eq]
+    apply Nat.add_lt_add m_lt n_lt
+  simp [Nat.mod_eq_of_lt d_lt]
+
+lemma B64.toNat_overflow {x y : B64} :
+    x + y < x ↔ 2 ^ 64 ≤ x.toNat + y.toNat := by
+  rw [B64.lt_iff_toNat_lt, B64.toNat_add]
+  by_cases h : x.toNat + y.toNat < 2 ^ 64
+  · rw [Nat.lo_eq_of_lt h]
+    apply iff_of_false <;> omega
+  · rw [not_lt] at h; apply iff_of_true _ h
+    have x_lt := @B64.toNat_lt x
+    have y_lt := @B64.toNat_lt y
+    rw [Nat.lo, Nat.add_mod_eq_add_sub x_lt y_lt h]
+    omega
+
+lemma ite_distrib {α β} {f : α → β} {p : Prop} [Decidable p] {a b : α} :
+    f (if p then a else b) = if p then f a else f b := by
+  by_cases h : p <;> simp [h]
+
+lemma ite_eq_ite_of_iff {α} {p q : Prop} [Decidable p] [Decidable q]
+    {a b c d : α} (pq : p ↔ q) (ac : a = c) (bd : b = d) :
+    (if p then a else b) = (if q then c else d) := by
+  rw [ac, bd]; by_cases h : p
+  · rw [if_pos h, if_pos (pq.mp h)]
+  · rw [if_neg h, if_neg (mt pq.mpr h)]
+
+lemma toB128_add (a b : Nat) : (a + b).toB128 = a.toB128 + b.toB128 := by
+  simp only [Nat.toB128, Nat.shiftRight_eq_div_pow]
+  rw [Nat.add_div (by omega)]; apply congr_arg₂ _ _ (toB64_add _ _)
+  simp only [toB64_add]; apply congr_arg₂ _ rfl
+  apply Eq.trans ite_distrib <| ite_eq_ite_of_iff _ rfl rfl
+  rw [← Nat.lo, ← Nat.lo, B64.toNat_overflow, toNat_toB64, toNat_toB64]
+
+lemma toB64_toNat (x : B64) : x.toNat.toB64 = x :=
+  UInt64.ofNat_toNat
+
+lemma B64.ofNat_eq_iff_mod_eq_toNat (a : Nat) (b : B64) :
+    a.toB64 = b ↔ a ↾ 64 = b.toNat :=
+  UInt64.ofNat_eq_iff_mod_eq_toNat a b
+
+lemma Nat.lo_lo {m n : Nat} : (m ↾ n) ↾ n = m ↾ n :=
+  Nat.mod_mod _ _
+
+lemma lo_toB64 (n : Nat) : (n ↾ 64).toB64 = n.toB64 := by
+  rw [← B64.toNat_inj, toNat_toB64, toNat_toB64, Nat.lo_lo]
+
+lemma Nat.or_lo {k m n : Nat} : (m ||| n) ↾ k = (m ↾ k) ||| (n ↾ k) :=
+  Nat.or_mod_two_pow
+
+lemma toB128_toNat (x : B128) : x.toNat.toB128 = x := by
+  simp only [B128.toNat, Nat.toB128]
+  apply congr_arg₂
+  · rw [Nat.shiftRight_or_distrib, Nat.shiftLeft_shiftRight]
+    rw [Nat.shiftRight_eq_zero _ _ B64.toNat_lt, Nat.or_zero, toB64_toNat]
+  · rw [← lo_toB64, Nat.or_lo, Nat.shl_lo_eq_zero_of_le (by omega)]
+    rw [Nat.zero_or, lo_toB64, toB64_toNat]
+
+lemma B128.toNat_inj (xs ys : B128) : xs.toNat = ys.toNat ↔ xs = ys := by
+  constructor <;> intro h
+  · rw [← toB128_toNat xs, ← toB128_toNat ys, h]
+  · simp [h]
+
+lemma lo_toB128 (n : Nat) : (n ↾ 128).toB128 = n.toB128 := by
+  rw [← B128.toNat_inj, toNat_toB128, toNat_toB128, Nat.lo_lo]
+
+--lemma toB128_eq_iff_mod_eq_toNat (a : Nat) (b : B128) :
+lemma toB128_eq_iff_lo_eq_toNat (a : Nat) (b : B128) :
+    a.toB128 = b ↔ a ↾ 128 = b.toNat := by
+  constructor <;> intro h
+  · rw [← h, toNat_toB128]
+  · rw [← B128.toNat_inj, ← h, toNat_toB128]
+
+lemma B128.zero_1 : (0 : B128).1 = 0 := rfl
+lemma B128.zero_2 : (0 : B128).2 = 0 := rfl
+
+lemma B128.sub_eq (x y : B128) :
+  x - y = ⟨(x.1 - y.1) - (if x.2 < y.2 then 1 else 0), x.2 - y.2⟩ := rfl
+
+lemma B256.sub_eq (x y : B256) :
+  x - y = ⟨(x.1 - y.1) - (if x.2 < y.2 then 1 else 0), x.2 - y.2⟩ := rfl
+
+def B128.add_eq (x y : B128) :
+  x + y = ⟨x.1 + y.1 + if x.2 + y.2 < x.2 then 1 else 0, x.2 + y.2⟩ := rfl
+
+def B256.add_eq (x y : B256) :
+  x + y = ⟨x.1 + y.1 + if x.2 + y.2 < x.2 then 1 else 0, x.2 + y.2⟩ := rfl
+
+lemma B128.zero_add (n : B128) : 0 + n = n := by
+  rw [B128.add_eq]; simp [B128.zero_1, B128.zero_2]
+
+lemma toB256_toNat (x : B256) : x.toNat.toB256 = x := by
+  simp only [B256.toNat, Nat.toB256]
+  apply congr_arg₂
+  · rw [Nat.shiftRight_or_distrib, Nat.shiftLeft_shiftRight]
+    rw [Nat.shiftRight_eq_zero _ _ B128.toNat_lt, Nat.or_zero, toB128_toNat]
+  · rw [← lo_toB128, Nat.or_lo, Nat.shl_lo_eq_zero_of_le (by omega)]
+    rw [Nat.zero_or, lo_toB128, toB128_toNat]
+
+theorem B256.toNat_inj (xs ys : B256) (eq : xs.toNat = ys.toNat) : xs = ys := by
+  rw [← toB256_toNat xs, ← toB256_toNat ys, eq]
+
+lemma B128.lt_or_eq_of_le {n m : B128} (h : n ≤ m) : n < m ∨ n = m := by
+  rcases h with h | h
+  · left; left; apply h
+  · rcases UInt64.lt_or_eq_of_le h.2 with h' | h'
+    · left; right; refine ⟨h.1, h'⟩
+    · right; apply Prod.ext h.1 h'
+
+lemma B256.lt_or_eq_of_le {n m : B256} (h : n ≤ m) : n < m ∨ n = m := by
+  rcases h with h | h
+  · left; left; apply h
+  · rcases B128.lt_or_eq_of_le h.2 with h' | h'
+    · left; right; refine ⟨h.1, h'⟩
+    · right; apply Prod.ext h.1 h'
+
+lemma B64.le_of_lt {a b : B64} : a < b → a ≤ b := UInt64.le_of_lt
+
+lemma B128.le_refl (x : B128) : x ≤ x := by
+  right; refine ⟨rfl, UInt64.le_refl _⟩
+
+lemma B256.le_refl (x : B256) : x ≤ x := by
+  right; refine ⟨rfl, B128.le_refl _⟩
+
+lemma B128.le_of_lt_or_eq {n m : B128} (h : n < m ∨ n = m) : n ≤ m := by
+  rcases h with (h | ⟨h, h'⟩) | h
+  · left; apply h
+  · right; refine' ⟨h, B64.le_of_lt h'⟩
+  · rw [h]; apply le_refl
+
+lemma B128.lt_iff (x y : B128) :
+  x < y ↔ (x.1 < y.1 ∨ (x.1 = y.1 ∧ x.2 < y.2)) := Iff.refl _
+
+lemma B256.lt_iff (x y : B256) :
+  x < y ↔ (x.1 < y.1 ∨ (x.1 = y.1 ∧ x.2 < y.2)) := Iff.refl _
+
+lemma B128.le_iff (x y : B128) :
+    x ≤ y ↔ (x.1 < y.1 ∨ (x.1 = y.1 ∧ x.2 ≤ y.2)) := Iff.refl _
+
+lemma B256.le_iff (x y : B256) :
+    x ≤ y ↔ (x.1 < y.1 ∨ (x.1 = y.1 ∧ x.2 ≤ y.2)) := Iff.refl _
+
+lemma B128.le_iff_lt_or_eq {n m : B128} : n ≤ m ↔ (n < m ∨ n = m) :=
+  ⟨B128.lt_or_eq_of_le, B128.le_of_lt_or_eq⟩
+
+lemma B128.le_or_gt (a b : B128) : a ≤ b ∨ a > b := by
+  simp [GT.gt]; rw [B128.le_iff, B128.lt_iff];
+  rcases UInt64.le_or_lt a.1 b.1 with h | h
+  · rcases UInt64.lt_or_eq_of_le h with h' | h'
+    · left; left; apply h'
+    · rcases UInt64.le_or_lt a.2 b.2 with h'' | h''
+      · left; right; refine ⟨h', h''⟩
+      · right; right; refine ⟨h'.symm, h''⟩
+  · right; left; apply h
+
+lemma B128.lt_or_ge (a b : B128) : a < b ∨ a ≥ b :=
+  Or.symm <| B128.le_or_gt _ _
+
+lemma B256.le_or_gt (a b : B256) : a ≤ b ∨ a > b := by
+  simp [GT.gt]; rw [B256.le_iff, B128.lt_iff];
+  rcases B128.le_or_gt a.1 b.1 with h | h
+  · rcases B128.lt_or_eq_of_le h with h' | h'
+    · left; left; apply h'
+    · rcases B128.le_or_gt a.2 b.2 with h'' | h''
+      · left; right; refine ⟨h', h''⟩
+      · right; right; refine ⟨h'.symm, h''⟩
+  · right; left; apply h
+
+lemma Nat.lt_of_lt_high {sz high low high' low' : Nat}
+    (h_high : high < high') (h_low : low < sz) :
+    high * sz + low < high' * sz + low' := by
+  rcases high' with _ | high'
+  · cases Nat.not_lt_zero _ h_high
+  · have h_le := Nat.le_of_lt_succ h_high
+    rw [Nat.succ_mul, Nat.add_assoc]
+    apply @Nat.add_lt_add_of_le_of_lt
+    · apply Nat.mul_le_mul_right _ h_le
+    · apply Nat.lt_add_right _ h_low
+
+lemma Nat.shl_or_lt_shl_or_of_left {k m n m' n' : Nat}
+    (m_lt_m' : m < m') (n_lt : n < 2 ^ k) (n'_lt : n' < 2 ^ k) :
+    m <<< k ||| n < m' <<< k ||| n' := by
+  rw [← Nat.add_eq_or two_pow_dvd_shl n_lt]
+  rw [← Nat.add_eq_or two_pow_dvd_shl n'_lt]
+  simp only [Nat.shiftLeft_eq]
+  apply lt_of_lt_high m_lt_m' n_lt
+
+lemma Nat.shl_or_lt_shl_or_of_right {k m n n' : Nat}
+    (n_lt : n < n') (n'_lt : n' < 2 ^ k) :
+    m <<< k ||| n < m <<< k ||| n' := by
+  rw [← Nat.add_eq_or two_pow_dvd_shl (lt_trans n_lt n'_lt)]
+  rw [← Nat.add_eq_or two_pow_dvd_shl n'_lt]
+  simp only [Nat.shiftLeft_eq]
+  rw [Nat.add_lt_add_iff_left]; apply n_lt
+
+lemma B128.toNat_lt_toNat {a b : B128} (h : a < b) :
+    a.toNat < b.toNat := by
+  rcases a with ⟨_, _⟩; rcases b with ⟨_, _⟩
+  rcases h with h | h <;> simp at h
+  · rw [B64.lt_iff_toNat_lt] at h
+    apply Nat.shl_or_lt_shl_or_of_left h B64.toNat_lt B64.toNat_lt
+  · rw [h.1]; apply Nat.shl_or_lt_shl_or_of_right _ B64.toNat_lt
+    rw [← B64.lt_iff_toNat_lt]; apply h.2
+
+lemma B128.toNat_le_toNat {a b : B128} (h : a ≤ b) : a.toNat ≤ b.toNat := by
+  rcases B128.lt_or_eq_of_le h with h | h
+  · apply Nat.le_of_lt <| B128.toNat_lt_toNat h
+  · rw [h]
+
+lemma B128.lt_of_toNat_lt_toNat {a b : B128} (lt : a.toNat < b.toNat) : a < b := by
+  rcases B128.le_or_gt b a with h | h
+  · cases not_le_of_gt lt <| B128.toNat_le_toNat h
+  · apply h
+
+lemma B128.lt_iff_toNat_lt_toNat {a b : B128} : a < b ↔ a.toNat < b.toNat := by
+  constructor
+  · apply B128.toNat_lt_toNat
+  · apply B128.lt_of_toNat_lt_toNat
+
+lemma B256.toNat_lt_toNat {a b : B256} (h : a < b) :
+    a.toNat < b.toNat := by
+  rcases a with ⟨_, _⟩; rcases b with ⟨_, _⟩
+  rcases h with h | h <;> simp at h
+  · rw [B128.lt_iff_toNat_lt_toNat] at h
+    apply Nat.shl_or_lt_shl_or_of_left h B128.toNat_lt B128.toNat_lt
+  · rw [h.1]; apply Nat.shl_or_lt_shl_or_of_right _ B128.toNat_lt
+    rw [← B128.lt_iff_toNat_lt_toNat]; apply h.2
+
+lemma B128.le_of_lt {a b : B128} (h : a < b) : a ≤ b := by
+  rcases h with h | h
+  · left; apply h
+  · right; refine' ⟨h.1, UInt64.le_of_lt h.2⟩
+
+lemma B256.le_of_lt {a b : B256} (h : a < b) : a ≤ b := by
+  rcases h with h | h
+  · left; apply h
+  · right; refine' ⟨h.1, B128.le_of_lt h.2⟩
+
+lemma B256.le_of_lt_or_eq {n m : B256} (h : n < m ∨ n = m) : n ≤ m := by
+  rcases h with (h | ⟨h, h'⟩) | h
+  · left; apply h
+  · right; refine' ⟨h, B128.le_of_lt h'⟩
+  · rw [h]; apply le_refl
+
+lemma B256.le_iff_lt_or_eq {n m : B256} : n ≤ m ↔ (n < m ∨ n = m) :=
+  ⟨B256.lt_or_eq_of_le, B256.le_of_lt_or_eq⟩
+
+lemma B256.toNat_le_toNat {a b : B256} (h : a ≤ b) : a.toNat ≤ b.toNat := by
+  rcases B256.lt_or_eq_of_le h with h | h
+  · apply Nat.le_of_lt <| B256.toNat_lt_toNat h
+  · rw [h]
+
+lemma B256.lt_of_toNat_lt_toNat {a b : B256} (lt : a.toNat < b.toNat) : a < b := by
+  rcases B256.le_or_gt b a with h | h
+  · cases not_le_of_gt lt <| B256.toNat_le_toNat h
+  · apply h
+
+lemma B256.lt_iff_toNat_lt_toNat {a b : B256} : a < b ↔ a.toNat < b.toNat := by
+  constructor
+  · apply B256.toNat_lt_toNat
+  · apply B256.lt_of_toNat_lt_toNat
+
+lemma B128.not_lt {a b : B128} : ¬ a < b ↔ b ≤ a := by
+  simp [B128.lt_iff, B128.le_iff]
+  rw [@Eq.comm _ a.1 b.1, @UInt64.le_iff_lt_or_eq b.1 a.1]
+  aesop
+
+lemma B128.lt_irrefl (x : B128) : ¬ x < x := by
+  intro h; rcases h with h | h <;> simp at h
+
+lemma B256.lt_irrefl (x : B256) : ¬ x < x := by
+  intro h; rcases h with h | h <;> simp [B128.lt_irrefl] at h
+
+lemma B256.not_lt {a b : B256} : ¬ a < b ↔ b ≤ a := by
+  simp [B256.lt_iff, B256.le_iff, B128.not_lt]
+  rw [@Eq.comm _ a.1 b.1, @B128.le_iff_lt_or_eq b.1 a.1]
+  by_cases h : b.1 < a.1 <;> simp [h] <;> intro h'
+  · rw [h'] at h; cases B128.lt_irrefl _ h
+  · apply Or.inl h'
+
+lemma B128.not_le {a b : B128} : ¬ a ≤ b ↔ b < a := by
+  rw [not_iff_comm, B128.not_lt]
+
+lemma B256.not_le {a b : B256} : ¬ a ≤ b ↔ b < a := by
+  rw [not_iff_comm, B256.not_lt]
+
+lemma B128.le_iff_toNat_le_toNat {a b : B128} : a ≤ b ↔ a.toNat ≤ b.toNat := by
+  rw [← not_iff_not, not_le, Nat.not_le, lt_iff_toNat_lt_toNat]
+
+lemma B256.le_iff_toNat_le_toNat {a b : B256} : a ≤ b ↔ a.toNat ≤ b.toNat := by
+  rw [← not_iff_not, not_le, Nat.not_le, lt_iff_toNat_lt_toNat]
+
+lemma B128.le_of_toNat_le_toNat {a b : B128} : a.toNat ≤ b.toNat → a ≤ b :=
+  B128.le_iff_toNat_le_toNat.mpr
+
+lemma B256.le_of_toNat_le_toNat {a b : B256} : a.toNat ≤ b.toNat → a ≤ b :=
+  B256.le_iff_toNat_le_toNat.mpr
+
+lemma Nat.lo_add_lo (m n k : ℕ) : (m ↾ k + n) ↾ k = (m + n) ↾ k :=
+  Nat.mod_add_mod _ _ _
+
+lemma B128.toNat_add (x y : B128) :
+    (x + y).toNat = (x.toNat + y.toNat) ↾ 128 := by
+  rw [B128.add_eq]; simp only [B128.toNat]
+  rw [Nat.shl_or_add_shl_or_lo_add B64.toNat_lt B64.toNat_lt]
+  apply congr_arg₂ _ (congr_arg₂ _ _ rfl) (B64.toNat_add _ _)
+  rw [B64.toNat_add, B64.toNat_add, Nat.lo_add_lo]
+  apply congr_arg₂ _ (congr_arg₂ _ rfl _) rfl
+  rw [← ite_not, @ite_distrib _ _ B64.toNat]
+  apply ite_eq_ite_of_iff _ rfl rfl
+  simp [B64.toNat_overflow]
+
+lemma B128.toNat_overflow {x y : B128} :
+    x + y < x ↔ 2 ^ 128 ≤ x.toNat + y.toNat := by
+  rw [B128.lt_iff_toNat_lt_toNat, B128.toNat_add]
+  by_cases h : x.toNat + y.toNat < 2 ^ 128
+  · rw [Nat.lo_eq_of_lt h]
+    apply iff_of_false <;> omega
+  · rw [_root_.not_lt] at h; apply iff_of_true _ h
+    have x_lt := @B128.toNat_lt x
+    have y_lt := @B128.toNat_lt y
+    rw [Nat.lo, Nat.add_mod_eq_add_sub x_lt y_lt h]
+    omega
+
+lemma toB256_add (a b : Nat) : (a + b).toB256 = a.toB256 + b.toB256 := by
+  simp only [Nat.toB256, Nat.shiftRight_eq_div_pow]
+  rw [Nat.add_div (by omega)]; apply congr_arg₂ _ _ (toB128_add _ _)
+  simp only [toB128_add]; apply congr_arg₂ _ rfl
+  apply Eq.trans ite_distrib <| ite_eq_ite_of_iff _ rfl rfl
+  rw [← Nat.lo, ← Nat.lo, B128.toNat_overflow, toNat_toB128, toNat_toB128]
+
+lemma B256.toNat_add (x y : B256) :
+    (x + y).toNat = (x.toNat + y.toNat) ↾ 256 := by
+  rw [B256.add_eq]; simp only [B256.toNat]
+  rw [Nat.shl_or_add_shl_or_lo_add B128.toNat_lt B128.toNat_lt]
+  apply congr_arg₂ _ (congr_arg₂ _ _ rfl) (B128.toNat_add _ _)
+  rw [B128.toNat_add, B128.toNat_add, Nat.lo_add_lo]
+  apply congr_arg₂ _ (congr_arg₂ _ rfl _) rfl
+  rw [← ite_not, @ite_distrib _ _ B128.toNat]
+  apply ite_eq_ite_of_iff _ rfl rfl
+  simp [B128.toNat_overflow]
+
+theorem B256.add_comm {xs ys : B256} : xs + ys = ys + xs := by
+  apply B256.toNat_inj
+  rw [B256.toNat_add, B256.toNat_add, Nat.add_comm]
+
+lemma toB32_toB64 (n : B32) : n.toB64.toB32 = n :=
+  UInt32.toUInt32_toUInt64 n
+
+def B256.toAdr (x : B256) : Adr := ⟨x.1.2.toB32, x.2⟩
+
+def Adr.toB256 (a : Adr) : B256 := ⟨⟨0, a.1.toB64⟩, a.2⟩
+
+lemma toAdr_toB256 (a : Adr) : a.toB256.toAdr = a := by
+  simp [Adr.toB256, B256.toAdr, toB32_toB64]
+
+theorem Adr.toB256_inj {x y : Adr} (eq : x.toB256 = y.toB256) : x = y := by
+  rw [← toAdr_toB256 x, ← toAdr_toB256 y, eq]
+
+
+lemma B64.toNat_sub {a b : B64} :
+    (a - b).toNat = (2 ^ 64 + a.toNat - b.toNat) ↾ 64 := by
+  apply Eq.trans (UInt64.toNat_sub _ _)
+  apply congr_arg₂ _ _ rfl
+  rw [Nat.sub_add_comm <| Nat.le_of_lt B64.toNat_lt]
+  rfl
+
+-- lemma Nat.add_sub_mod_eq_sub {k m n : Nat}
+--     (hm : m < k) (h : n ≤ m) : (k + m - n) % k = m - n := by
+--   rw [Nat.add_sub_assoc h, Nat.add_mod_left, Nat.mod_eq_of_lt]
+--   apply lt_of_le_of_lt (Nat.sub_le _ _) hm
+--
+-- lemma Nat.add_sub_mod_eq_add_sub {k m n : Nat}
+--     (hn : n ≤ k) (h : m < n) : (k + m - n) % k = k + m - n := by
+--   rw [Nat.mod_eq_of_lt]
+--   apply Nat.sub_lt_right_of_lt_add (by omega)
+--   apply Nat.add_lt_add_left h
+
+lemma Nat.add_mul_self_mod (x y z : ℕ) : (x + y * z) % z = x % z := by
+  induction y with
+  | zero => simp
+  | succ y ih => rw [succ_mul, ← Nat.add_assoc, add_mod_right, ih]
+
+lemma Nat.sub_mod_eq_sub_mod_right {a d c b : Nat}
+    (eq : a % d = b % d) (le_a : c ≤ a) (le_b : c ≤ b) :
+    (a - c) % d = (b - c) % d := by
+  rcases d with _ | d
+  · simp at *; rw [eq]
+  · rw [← add_mul_self_mod _ c, ← add_mul_self_mod (b - c) c]
+    rw [← Nat.sub_add_comm le_a, ← Nat.sub_add_comm le_b]
+    rw [Nat.add_sub_assoc (Nat.le_mul_of_pos_right _ (by omega))]
+    rw [Nat.add_sub_assoc (Nat.le_mul_of_pos_right _ (by omega))]
+    apply Nat.add_mod_eq_add_mod_right _ eq
+
+
+  -- by_cases h : d = 0
+  -- · simp [h] at eq; rw [eq]
+  -- · rw [← add_mul_self_mod _ c d]
+  --   rw [← add_mul_self_mod (b - c) c d]
+  --   rw [← Nat.sub_add_comm le_a]
+  --   rw [← Nat.sub_add_comm le_b]
+  --   have hd : 0 < d := by
+  --     cases d
+  --     · cases h rfl
+  --     · simp
+  --   rw [Nat.add_sub_assoc (Nat.le_mul_of_pos_right _ hd)]
+  --   rw [Nat.add_sub_assoc (Nat.le_mul_of_pos_right _ hd)]
+  --   apply Nat.add_mod_eq_add_mod_right _ eq
+
+lemma B64.toNat_zero : B64.toNat 0 = 0 := rfl
+lemma B64.toNat_one : B64.toNat 1 = 1 := rfl
+
+lemma Nat.two_pow_add_lo (x y : Nat) : (2 ^ x + y) ↾ x = y ↾ x :=
+  Nat.add_mod_left _ _
+
+lemma B128.toNat_sub {a b : B128} :
+    (a - b).toNat = (2 ^ 128 + a.toNat - b.toNat) ↾ 128 := by
+  rw [B128.sub_eq]; simp only [B128.toNat]
+  rw [Nat.add_shl_or_sub_shl_or_lo_add B64.toNat_lt B64.toNat_lt B64.toNat_lt]
+  apply congr_arg₂ _ (congr_arg₂ _ _ rfl) B64.toNat_sub
+  simp only [B64.toNat_sub]
+  rw [@ite_distrib _ _ B64.toNat, B64.toNat_one, B64.toNat_zero]
+  rw [← ite_eq_ite_of_iff B64.lt_iff_toNat_lt rfl rfl]
+  apply Nat.sub_mod_eq_sub_mod_right
+  · rw [Nat.add_mod_left]; apply Nat.lo_lo
+  · split <;> omega
+  · have _ := @B64.toNat_lt b.1; split <;> omega
+
+lemma B128.toNat_zero : B128.toNat 0 = 0 := rfl
+lemma B128.toNat_one : B128.toNat 1 = 1 := rfl
+
+lemma B256.toNat_sub (a b : B256) :
+    (a - b).toNat = (2 ^ 256 + a.toNat - b.toNat) ↾ 256 := by
+  rw [B256.sub_eq]; simp only [B256.toNat]
+  rw [Nat.add_shl_or_sub_shl_or_lo_add B128.toNat_lt B128.toNat_lt B128.toNat_lt]
+  apply congr_arg₂ _ (congr_arg₂ _ _ rfl) B128.toNat_sub
+  simp only [B128.toNat_sub]
+  rw [@ite_distrib _ _ B128.toNat, B128.toNat_one, B128.toNat_zero]
+  rw [← ite_eq_ite_of_iff B128.lt_iff_toNat_lt_toNat rfl rfl]
+  apply Nat.sub_mod_eq_sub_mod_right
+  · rw [Nat.add_mod_left]; apply Nat.lo_lo
+  · split <;> omega
+  · have _ := @B128.toNat_lt b.1; split <;> omega
+
+lemma B128.lt_asymm {a b : B128} (h : a < b) : ¬ b < a := by
+  intro h'; rcases h with h | h <;> rcases h' with h' | h'
+  · cases UInt64.lt_asymm h h'
+  · rw [h'.1] at h; cases UInt64.lt_irrefl _ h
+  · rw [h.1] at h'; cases UInt64.lt_irrefl _ h'
+  · cases UInt64.lt_asymm h.2 h'.2
+
+lemma B256.lt_asymm {a b : B256} (h : a < b) : ¬ b < a := by
+  intro h'; rcases h with h | h <;> rcases h' with h' | h'
+  · cases B128.lt_asymm h h'
+  · rw [h'.1] at h; cases B128.lt_irrefl _ h
+  · rw [h.1] at h'; cases B128.lt_irrefl _ h'
+  · cases B128.lt_asymm h.2 h'.2
+
+lemma B128.lt_iff_le_not_ge {a b : B128} : a < b ↔ a ≤ b ∧ ¬b ≤ a := by
+  rw [not_le, ← not_lt]; simp; apply lt_asymm
+
+lemma B256.lt_iff_le_not_ge {a b : B256} : a < b ↔ a ≤ b ∧ ¬b ≤ a := by
+  rw [not_le, ← not_lt]; simp; apply lt_asymm
+
+lemma B128.lt_trans {a b c : B128} (ab : a < b) (bc : b < c) : a < c := by
+  rcases ab with ab | ab <;> rcases bc with bc | bc
+  · left; apply UInt64.lt_trans ab bc
+  · left; rw [← bc.1]; exact ab
+  · left; rw [ab.1]; exact bc
+  · right; refine ⟨Eq.trans ab.1 bc.1, UInt64.lt_trans ab.2 bc.2⟩
+
+lemma B128.le_trans {a b c : B128} (ab : a ≤ b) (bc : b ≤ c) : a ≤ c := by
+  rcases ab with ab | ab <;> rcases bc with bc | bc
+  · left; apply UInt64.lt_trans ab bc
+  · left; rw [← bc.1]; exact ab
+  · left; rw [ab.1]; exact bc
+  · right; refine ⟨Eq.trans ab.1 bc.1, UInt64.le_trans ab.2 bc.2⟩
+
+lemma B256.le_trans {a b c : B256} (ab : a ≤ b) (bc : b ≤ c) : a ≤ c := by
+  rcases ab with ab | ab <;> rcases bc with bc | bc
+  · left; apply B128.lt_trans ab bc
+  · left; rw [← bc.1]; exact ab
+  · left; rw [ab.1]; exact bc
+  · right; refine ⟨Eq.trans ab.1 bc.1, B128.le_trans ab.2 bc.2⟩
+
+instance : Preorder B128 where
+  le_refl := B128.le_refl
+  le_trans _ _ _ := B128.le_trans
+  lt := B128.LT
+  lt_iff_le_not_ge _ _ := B128.lt_iff_le_not_ge
+
+instance : Preorder B256 where
+  le_refl := B256.le_refl
+  le_trans _ _ _ := B256.le_trans
+  lt := B256.LT
+  lt_iff_le_not_ge _ _ := B256.lt_iff_le_not_ge
+
+lemma B128.le_antisymm {a b : B128} : a ≤ b → b ≤ a → a = b := by
+  intro h₁ h₂; rw [le_iff_lt_or_eq] at h₁ h₂
+  rcases h₁ with h₁ | h₁
+  · rcases h₂ with h₂ | h₂
+    · cases B128.lt_asymm h₁ h₂
+    · exact h₂.symm
+  · exact h₁
+
+lemma B256.le_antisymm {a b : B256} : a ≤ b → b ≤ a → a = b := by
+  intro h₁ h₂; rw [le_iff_lt_or_eq] at h₁ h₂
+  rcases h₁ with h₁ | h₁
+  · rcases h₂ with h₂ | h₂
+    · cases B256.lt_asymm h₁ h₂
+    · exact h₂.symm
+  · exact h₁
+
+instance : PartialOrder B128 where
+  le_antisymm _ _ := B128.le_antisymm
+
+instance : PartialOrder B256 where
+  le_antisymm _ _ := B256.le_antisymm
+
+lemma B128.le_total (m n : B128) : m ≤ n ∨ n ≤ m := by
+  rcases B128.le_or_gt m n with h | h
+  · left; apply h
+  · right; simp [GT.gt] at h; apply B128.le_of_lt h
+
+lemma B256.le_total (m n : B256) : m ≤ n ∨ n ≤ m := by
+  rcases B256.le_or_gt m n with h | h
+  · left; apply h
+  · right; simp [GT.gt] at h; apply B256.le_of_lt h
+
+instance : DecidableLT B128 :=
+  fun a b => by rw [B128.lt_iff]; infer_instance
+
+instance : DecidableLE B128 :=
+  fun a b => by rw [B128.le_iff]; infer_instance
+
+instance : DecidableEq B128 :=
+  fun a b => by rw [Prod.ext_iff]; infer_instance
+
+instance : DecidableLT B256 :=
+  fun a b => by rw [B256.lt_iff]; infer_instance
+
+instance : DecidableLE B256 :=
+  fun a b => by rw [B256.le_iff]; infer_instance
+
+instance : DecidableEq B256 :=
+  fun a b => by rw [Prod.ext_iff]; infer_instance
+
+instance : Ord B128 where
+  compare a b := compareOfLessAndEq a b
+
+instance : Ord B256 where
+  compare a b := compareOfLessAndEq a b
+
+instance : LinearOrder B128 where
+  le_total := B128.le_total
+  toDecidableLE := instDecidableLEB128
+
+instance : LinearOrder B256 where
+  le_total := B256.le_total
+  toDecidableLE := instDecidableLEB256
+
+def Adr.LE (x y : Adr) : Prop :=
+  x.1 < y.1 ∨ (x.1 = y.1 ∧ x.2 ≤ y.2)
+instance : @LE Adr := ⟨Adr.LE⟩
+instance {x y : Adr} : Decidable (x ≤ y) := instDecidableOr
+
+lemma Adr.le_iff (x y : Adr) :
+  x ≤ y ↔ (x.1 < y.1 ∨ (x.1 = y.1 ∧ x.2 ≤ y.2)) := Iff.refl _
+
+lemma Adr.le_refl (x : Adr) : x ≤ x := by
+  right; refine ⟨rfl, B128.le_refl _⟩
+
+lemma Adr.le_trans {a b c : Adr} (ab : a ≤ b) (bc : b ≤ c) : a ≤ c := by
+  rcases ab with ab | ab <;> rcases bc with bc | bc
+  · left; apply UInt32.lt_trans ab bc
+  · left; rw [← bc.1]; exact ab
+  · left; rw [ab.1]; exact bc
+  · right; refine ⟨Eq.trans ab.1 bc.1, B128.le_trans ab.2 bc.2⟩
+
+def Adr.LT (x y : Adr) : Prop := x.1 < y.1 ∨ (x.1 = y.1 ∧ x.2 < y.2)
+instance : @LT Adr := ⟨Adr.LT⟩
+instance {x y : Adr} : Decidable (x < y) := instDecidableOr
+
+lemma Adr.lt_iff (x y : Adr) :
+  x < y ↔ (x.1 < y.1 ∨ (x.1 = y.1 ∧ x.2 < y.2)) := Iff.refl _
+
+lemma Adr.lt_iff_le_not_ge {a b : Adr} : a < b ↔ a ≤ b ∧ ¬b ≤ a := by
+  constructor <;> intro h
+  · rcases h with h | h
+    · refine' ⟨.inl h, not_or_intro (UInt32.lt_asymm h) _⟩
+      apply not_and_of_not_left _ <| Ne.symm <| UInt32.ne_of_lt h
+    · refine' ⟨.inr ⟨h.1, B128.le_of_lt h.2⟩, not_or_intro _ _⟩
+      · rw [h.1]; apply UInt32.lt_irrefl
+      · apply not_and_of_not_right; rw [B128.not_le]; apply h.2
+  · rcases h with ⟨h | ⟨h1, h2⟩, h'⟩
+    · apply Or.inl h
+    · rcases not_or.mp h' with ⟨h1', h2'⟩
+      right; refine' ⟨h1, B128.lt_iff_le_not_ge.mpr ⟨h2, not_and.mp h2' h1.symm⟩⟩
+
+instance : Preorder Adr where
+  le_refl := Adr.le_refl
+  le_trans _ _ _ := Adr.le_trans
+  lt := Adr.LT
+  lt_iff_le_not_ge _ _ := Adr.lt_iff_le_not_ge
+
+lemma Adr.le_antisymm {a b : Adr} : a ≤ b → b ≤ a → a = b := by
+  intro h₁ h₂
+  rcases h₁ with h₁ | h₁ <;> rcases h₂ with h₂ | h₂
+  · cases lt_asymm h₁ h₂
+  · cases UInt32.ne_of_lt h₁ h₂.1.symm
+  · cases UInt32.ne_of_lt h₂ h₁.1.symm
+  · exact Prod.ext h₁.1 <| B128.le_antisymm h₁.2 h₂.2
+
+instance : PartialOrder Adr where
+  le_antisymm _ _ := Adr.le_antisymm
+
+lemma Adr.le_total (m n : Adr) : m ≤ n ∨ n ≤ m := by
+  by_cases h : m.1 < n.1
+  · left; left; exact h
+  · rw [not_lt, UInt32.le_iff_lt_or_eq] at h
+    rcases h with h | h
+    · right; left; exact h
+    · rcases B128.le_total m.2 n.2 with h' | h'
+      · left; right; refine ⟨h.symm, h'⟩
+      · right; right; refine ⟨h, h'⟩
+
+instance : DecidableLT Adr :=
+  fun a b => by rw [Adr.lt_iff]; infer_instance
+
+instance : DecidableLE Adr :=
+  fun a b => by rw [Adr.le_iff]; infer_instance
+
+instance : DecidableEq Adr :=
+  fun a b => by rw [Prod.ext_iff]; infer_instance
+
+instance : Ord Adr where
+  compare a b := compareOfLessAndEq a b
+
+instance : LinearOrder Adr where
+  le_total := Adr.le_total
+  toDecidableLE := by infer_instance
+
+lemma Adr.lt_asymm {a b : Adr} (h : a < b) : ¬ b < a := by
+  intro h'; rcases h with h | h <;> rcases h' with h' | h'
+  · cases UInt32.lt_asymm h h'
+  · rw [h'.1] at h; cases UInt32.lt_irrefl _ h
+  · rw [h.1] at h'; cases UInt32.lt_irrefl _ h'
+  · cases B128.lt_asymm h.2 h'.2
+
+lemma Adr.lt_irrefl (x : Adr) : ¬ x < x := by
+  intro h; rcases h with h | h <;> simp at h
+
+
+-- lemma B128.toNat_sub (a b : B128) :
+--     (a - b).toNat = (2 ^ 128 + a.toNat - b.toNat) % 2 ^ 128 := by
+--   rw [B128.sub_eq]; simp only [B128.toNat]
+--   rw [
+--     @Nat.concat_modsub_concat 64 64 a.1.toNat a.2.toNat b.1.toNat b.2.toNat
+--       (UInt64.toNat_lt_size _)
+--       (UInt64.toNat_lt_size _)
+--       (UInt64.toNat_lt_size _)
+--   ]
+--   apply congr_arg₂ _ _ (by rw [UInt64.toNat_sub'])
+--   apply congr_arg₂ _ _ rfl
+--   by_cases h : a.2 < b.2
+--   · rw [if_pos h, if_pos (UInt64.lt_iff_toNat_lt.mp h)]; clear h
+--     rw [UInt64.toNat_sub', UInt64.toNat_one, UInt64.toNat_sub']
+--     rcases _root_.le_or_gt b.1.toNat a.1.toNat with h | h
+--     · rw [Nat.add_sub_mod_eq_sub (UInt64.toNat_lt_pow _) h]
+--       rw [← Nat.add_sub_assoc h]
+--     · rw [Nat.add_sub_mod_eq_add_sub (Nat.le_of_lt (UInt64.toNat_lt_pow b.1)) h]
+--       have h' : 2 ^ 64 + UInt64.toNat a.1 - UInt64.toNat b.1 < 2 ^ 64 := by
+--         apply Nat.sub_lt_right_of_lt_add
+--         · apply Nat.le_of_lt
+--           apply lt_of_lt_of_le (UInt64.toNat_lt_size _) (Nat.le_add_right _ _)
+--         · apply Nat.add_lt_add_left h
+--       have h'' : 1 ≤ 2 ^ 64 + UInt64.toNat a.1 - UInt64.toNat b.1 := by
+--         apply Nat.succ_le_of_lt
+--         apply
+--           lt_of_lt_of_le
+--             (Nat.zero_lt_sub_of_lt (UInt64.toNat_lt_pow b.1))
+--             (by omega)
+--       rw [Nat.add_sub_mod_eq_sub h' h'']
+--       rw [← Nat.sub_add_eq, Nat.add_sub_mod_eq_add_sub]
+--       · apply Nat.succ_le_of_lt <| UInt64.toNat_lt_pow _
+--       · apply lt_trans h <| Nat.lt_succ_self _
+--   · rw [if_neg h, if_neg (mt UInt64.lt_iff_toNat_lt.mpr h)]
+--     rw [Nat.sub_zero, UInt64.sub_zero, UInt64.toNat_sub']
+
+theorem B256.sub_add_cancel {x y : B256} : x - y + y = x := by
+  apply B256.toNat_inj
+  simp only [B256.toNat_add, B256.toNat_sub]
+  have x_lt : x.toNat < 2 ^ 256 := B256.toNat_lt _
+  have y_lt : y.toNat < 2 ^ 256 := B256.toNat_lt _
+  revert x_lt; revert y_lt
+  generalize x.toNat = x, y.toNat = y
+  intros y_lt x_lt
+  by_cases h : x < y
+  · rw [@Nat.lo_eq_of_lt (2 ^ 256 + x - y) _ (by omega)]
+    rw [Nat.sub_add_cancel (by omega)]
+    rw [Nat.two_pow_add_lo, Nat.lo_eq_of_lt x_lt]
+  · rw [Nat.not_lt] at h
+    rw [Nat.add_sub_assoc h, Nat.two_pow_add_lo]
+    rw [Nat.lo_eq_of_lt (by {rw [Nat.lo]; omega})]
+    rw [Nat.lo_eq_of_lt (by omega)]
+    apply Nat.sub_add_cancel h
+
+lemma toAdr_toNat (a : Adr) : a.toNat.toAdr = a := by
   simp only [Nat.toAdr, Adr.toNat]
-  have h_high :
-      ((a.high.toNat * 2 ^ 128 + a.mid.toNat * 2 ^ 64 + a.low.toNat) / 2 ^ 128).toUInt32 = a.high := by
-    rw [Nat.add_assoc, Nat.add_div_of_dvd_of_lt]
-    · have h_lt := B64.toNat_mul_add_toNat_lt_size a.mid a.low
-      rw [Nat.div_eq_of_lt h_lt, Nat.mul_div_cancel _ (Nat.two_pow_pos _)]
-      apply UInt32.ofNat_toNat
-    · apply Nat.dvd_mul_left
-    · apply B64.toNat_mul_add_toNat_lt_size
-  rw [h_high]; clear h_high
-  have h_mid :
-      ((a.high.toNat * 2 ^ 128 + a.mid.toNat * 2 ^ 64 + a.low.toNat) / 2 ^ 64).toUInt64 = a.mid := by
-    rw [Nat.add_div_of_dvd_of_lt _ (UInt64.toNat_lt_size _)]
-    · rw [Nat.div_eq_of_lt <| UInt64.toNat_lt_size a.low, Nat.add_zero]
-      have h_dvd : 2 ^ 64 ∣ UInt32.toNat a.high * 2 ^ 128 := by
-        rw [aux]; apply Nat.dvd_mul_left
-      rw [Nat.add_div_of_dvd_of_dvd h_dvd (Nat.dvd_mul_left _ _) (Nat.two_pow_pos _)]
-      rw [Nat.mul_div_cancel _ (Nat.two_pow_pos _)]
-      rw [aux, Nat.mul_div_cancel _ (Nat.two_pow_pos _)]
-      simp
-    · rw [aux]; apply Nat.dvd_add <;> apply Nat.dvd_mul_left
-  rw [h_mid]; clear h_mid
-  simp
+  apply Prod.ext <;> simp
+  · rw [Nat.shiftRight_or_distrib, Nat.shiftLeft_shiftRight]
+    rw [Nat.shiftRight_eq_zero _ _ B128.toNat_lt, Nat.or_zero]
+    apply toB32_toNat
+  · rw [toB128_or]
+    have eq : (a.1.toNat <<< 128).toB128 = 0 := by
+      rw [toB128_eq_iff_lo_eq_toNat]
+      rw [Nat.shl_lo_eq_zero_of_le (by omega)]
+      rfl
+    rw [eq, B128.zero_or]
+    apply toB128_toNat
 
-def Adr.ordering : Adr → Adr → Ordering
-  | ⟨xh, xm, xl⟩, ⟨yh, ym, yl⟩ =>
-    match compare xh yh with
-    | .eq =>
-      match compare xm ym with
-      | .eq => compare xl yl
-      | o => o
-    | o => o
+-- lemma Adr'.toAdr_toNat (a : Adr') : a.toNat.toAdr' = a := by
+--   have aux : ∀ x : Nat, x * (2 ^ 128) = x * (2 ^ 64) * (2 ^ 64) := by
+--     intro x; rw [Nat.mul_assoc]
+--   simp only [Nat.toAdr', Adr'.toNat]
+--   have h_high :
+--       ((a.high.toNat * 2 ^ 128 + a.mid.toNat * 2 ^ 64 + a.low.toNat) / 2 ^ 128).toUInt32 = a.high := by
+--   -- rw [Nat.add_assoc, Nat.add_div_of_dvd_of_lt]
+--   -- · have h_lt := B64.toNat_mul_add_toNat_lt_size a.mid a.low
+--   --   rw [Nat.div_eq_of_lt h_lt, Nat.mul_div_cancel _ (Nat.two_pow_pos _)]
+--   --   apply UInt32.ofNat_toNat
+--   -- · apply Nat.dvd_mul_left
+--   -- · apply B64.toNat_mul_add_toNat_lt_size
+--     sorry
+--   rw [h_high]; clear h_high
+--   have h_mid :
+--       ((a.high.toNat * 2 ^ 128 + a.mid.toNat * 2 ^ 64 + a.low.toNat) / 2 ^ 64).toUInt64 = a.mid := by
+--     rw [Nat.add_div_of_dvd_of_lt _ (UInt64.toNat_lt_size _)]
+--
+--
+--     · rw [Nat.div_eq_of_lt <| UInt64.toNat_lt_size a.low, Nat.add_zero]
+--       have h_dvd : 2 ^ 64 ∣ UInt32.toNat a.high * 2 ^ 128 := by
+--         rw [aux]; apply Nat.dvd_mul_left
+--       rw [Nat.add_div_of_dvd_of_dvd h_dvd (Nat.dvd_mul_left _ _) (Nat.two_pow_pos _)]
+--       rw [Nat.mul_div_cancel _ (Nat.two_pow_pos _)]
+--
+--       rw [aux, Nat.mul_div_cancel _ (Nat.two_pow_pos _)]
+--
+--       simp
+--
+--     · rw [aux]; apply Nat.dvd_add <;> apply Nat.dvd_mul_left
+--   rw [h_mid]; clear h_mid
+--   simp
 
-instance : Ord Adr := ⟨Adr.ordering⟩
+-- def Adr.compare (a b : Adr) : Ordering :=
+--   match Ord.compare a.1 b.1 with
+--   | .eq => Ord.compare a.2 b.2
+--   | o => o
 
-def Adr.toHex (a : Adr) : String :=
-  a.high.toHex ++ a.mid.toHex ++ a.low.toHex
+-- def Adr.compare : Adr → Adr → Ordering
+--   | ⟨xh, xm, xl⟩, ⟨yh, ym, yl⟩ =>
+--     match Ord.compare xh yh with
+--     | .eq =>
+--       match Ord.compare xm ym with
+--       | .eq => Ord.compare xl yl
+--       | o => o
+--     | o => o
+
+--instance : Ord Adr := {compare := Adr.compare}
+
+def Adr.toHex (a : Adr) : String := a.1.toHex ++ a.2.toHex
 
 instance : ToString Adr := ⟨Adr.toHex⟩
 
@@ -131,6 +940,17 @@ def String.dropZeroes (s : String) : String :=
 
 abbrev Stor := Std.TreeMap B256 B256 compare
 
+def Stor.empty : Stor := Std.TreeMap.empty
+
+lemma Std.TreeMap.eq_empty_of_isEmpty {α : Type u} {β : Type v}
+    {cmp : α → α → Ordering} {t : Std.TreeMap α β cmp} (h : t.isEmpty = true) :
+    t = Std.TreeMap.empty := by
+  rcases t with ⟨⟨dt, wf⟩⟩
+  simp [Std.TreeMap.isEmpty, Std.DTreeMap.isEmpty] at h
+  cases dt
+  · simp [Std.DTreeMap.Internal.Impl.isEmpty] at h
+  · rfl
+
 def Stor.toStrings (s : Stor) : List String :=
   let kvs := s.toArray.toList
   let kvToStrings : B256 × B256 → List String :=
@@ -139,11 +959,15 @@ def Stor.toStrings (s : Stor) : List String :=
 
 instance : ToString Stor := ⟨String.joinln ∘ Stor.toStrings⟩
 
+@[ext]
 structure Acct where
   (nonce : B64)
   (bal : B256)
   (stor : Stor)
   (code : ByteArray)
+
+def Acct.withBal (a : Acct) (bal : B256) : Acct :=
+  {a with bal := bal}
 
 def Acct.toStrings (s : String) (a : Acct) : List String :=
   let codeStrings : List String :=
@@ -181,8 +1005,7 @@ def B8L.toAdr? : B8L → Option Adr
 
 def Hex.toAdr? (hx : String) : Option Adr := Hex.toB8L hx >>= B8L.toAdr?
 
-def Adr.toB8L (a : Adr) : B8L :=
-  a.high.toB8L ++ a.mid.toB8L ++ a.low.toB8L
+def Adr.toB8L (a : Adr) : B8L := a.1.toB8L ++ a.2.toB8L
 
 inductive Rinst : Type
   | add -- 0x01 / 2 / 1 / addition operation.
